tools/local-dafny.sh
@@ -5,6 +5,7 @@
 
 
 echo "NOTE: this will use the /noNLarith flag! If you're working on a file where nonlinear arith is allowed use tools/local-dafny-nonlinear.sh"
+echo "NOTE: since it's okay to park in the middle of the street with my blinkers on, jonh added /compile:0"
 DIR="$( cd "$( dirname "${BASH_SOURCE[0]}" )" >/dev/null 2>&1 && pwd )"
 set -x
-$DIR/../.dafny/bin/dafny "$@" /induction:1 /noNLarith
+$DIR/../.dafny/bin/dafny "$@" /induction:1 /noNLarith /compile:0
